verified

CBS.c
@@ -16,15 +16,16 @@ bool CBS_cbs_get_u(CBS_cbs_t *cbs, uint32_t *out, uint32_t num)
   uint32_t len = scrut0.len;
   if (len >= num)
   {
+    out[0U] = (uint32_t)0U;
     for (uint32_t i = (uint32_t)0U; i < num; i = i + (uint32_t)1U)
     {
       CBS_cbs_t scrut = cbs0;
       uint8_t *data = scrut.data;
       uint8_t bi = data[i];
-      uint32_t uu____211 = out[0U];
-      uint32_t uu____210 = uu____211 << (uint32_t)8U;
-      uint32_t uu____209 = uu____210 | (uint32_t)bi;
-      out[0U] = uu____209;
+      uint32_t lo = (uint32_t)bi;
+      uint32_t uu____225 = out[0U];
+      uint32_t hi = uu____225 << (uint32_t)8U;
+      out[0U] = hi | lo;
     }
     return true;
   }
@@ -41,8 +42,8 @@ bool CBS_cbs_get_u8(CBS_cbs_t *cbs, uint8_t *out)
   {
     CBS_cbs_t scrut = cbs0;
     uint8_t *data = scrut.data;
-    uint8_t uu____262 = data[0U];
-    out[0U] = uu____262;
+    uint8_t uu____280 = data[0U];
+    out[0U] = uu____280;
     return true;
   }
   else
