CBS.fst
@@ -6,11 +6,10 @@ open FStar.HyperStack.ST
 open FStar.Buffer
 open FStar.Mul
 
-module ST = FStar.HyperStack.ST
-
 module U8 = FStar.UInt8
 module U16 = FStar.UInt16
 module U32 = FStar.UInt32
+module ST = FStar.HyperStack.ST
 
 #reset-options "--max_fuel 5 --z3rlimit 100"
 
@@ -23,49 +22,70 @@ let u8_to_u32 n = FStar.Int.Cast.uint8_to_uint32 n
 [@ "substitute"] private
 let u32_to_u16 n = FStar.Int.Cast.uint32_to_uint16 n
 
+
+// TODO get rid of seq.last
 private // TODO move to CBS.Spec ?
 let rec big_endian (b:seq U8.t) : Tot (n:nat) (decreases (Seq.length b)) =
   let open FStar.Seq in
     if length b = 0 then 0
     else U8.v (last b) + pow2 8 * big_endian (slice b 0 (length b - 1))
 
+
+// bool cbs_get_u(cbs_t *cbs, uint32_t *out, uint32_t num)
+// TODO check that num < 5
 val cbs_get_u :
-  cbs: buffer cbs_t{length cbs = 1} ->
-  out: buffer U32.t{length out = 1} ->
+  cbs: buffer cbs_t{length cbs = 1} -> // TODO cbs_p ?
+  out: buffer U32.t{length out = 1 /\ disjoint out cbs} -> // TODO uint32_p ?
   num: U32.t{U32.(v num > 0 /\ v num < 5)} ->
   ST bool
-  (requires (fun h -> live h out /\ live h cbs /\ live h (get h cbs 0).data))
+  (requires (fun h -> live h out /\ live h cbs /\ live h (get h cbs 0).data
+    /\ disjoint out (get h cbs 0).data /\ disjoint cbs (get h cbs 0).data // TODO
+  ))
   (ensures (fun h0 r h1 -> live h0 out /\ live h1 out /\ modifies_1 out h0 h1 /\
     (let cbs0 = get h0 cbs 0 in
       // Return false if there aren't enough bytes.
-      r == U32.(v cbs0.len >= v num) //\
+      r == U32.(v cbs0.len >= v num) /\
       // If there are, check the result.
-      //(r ==> U32.v (get h1 out 0) == big_endian (slice (as_seq h0 cbs0.data) 0 (U32.v num)))
+      (r ==> U32.v (get h1 out 0) == big_endian (slice (as_seq h0 cbs0.data) 0 (U32.v num))) // TODO
     )))
 
 let cbs_get_u cbs out num =
   let cbs0 = cbs.(0ul) in
   let h0 = ST.get() in
   if U32.(cbs0.len >=^ num) then (
-    let inv = (fun h _ -> live h out /\ live h cbs0.data /\ modifies_1 out h0 h) in
+    let inv = (fun h i -> live h out /\ live h cbs0.data /\ modifies_1 out h0 h
+      /\ 0 <= i /\ i <= U32.v num // TODO comments
+      /\ U32.v (get h out 0) < pow2 (i * 8)
+      /\ U32.v (get h out 0) == big_endian (slice (as_seq h0 cbs0.data) 0 i)
+    ) in
     let f (i:U32.t{U32.(v 0ul <= v i /\ v i < v num)}) :
       Stack unit
-        (requires (fun h -> live h out /\ live h cbs0.data))
-        (ensures (fun h0 _ h1 -> modifies_1 out h0 h1))
+        (requires (fun h -> inv h (U32.v i)))
+        (ensures (fun h0 _ h1 -> inv h1 (U32.v i + 1)))
       = let bi = cbs0.data.(i) in
-        out.(0ul) <- U32.((out.(0ul) <<^ 8ul) |^ u8_to_u32 bi)
+        let lo = u8_to_u32 bi in
+        Math.Lemmas.pow2_plus 8 8;
+        Math.Lemmas.pow2_plus 8 16;
+        let hi = U32.(out.(0ul) <<^ 8ul) in
+        UInt.logor_disjoint #32 (U32.v hi) (U32.v lo) 8;
+        out.(0ul) <- U32.(hi |^ lo)
     in
+    out.(0ul) <- 0ul;
     C.Loops.for 0ul num inv f;
     true
   ) else (
     false
   )
 
+
+// bool cbs_get_u8(cbs_t *cbs, uint8_t *out)
 val cbs_get_u8 :
   cbs: buffer cbs_t{length cbs = 1} ->
-  out: buffer U8.t{length out = 1} ->
+  out: buffer U8.t{length out = 1 /\ disjoint out cbs} ->
   ST bool
-  (requires (fun h -> live h cbs /\ live h out /\ live h (get h cbs 0).data))
+  (requires (fun h -> live h cbs /\ live h out /\ live h (get h cbs 0).data
+    /\ disjoint out (get h cbs 0).data /\ disjoint cbs (get h cbs 0).data
+  ))
   (ensures (fun h0 r h1 -> live h1 out /\ modifies_1 out h0 h1 /\
     (let cbs0 = get h0 cbs 0 in
       // Return false if there aren't enough bytes.
@@ -83,17 +103,21 @@ let cbs_get_u8 cbs out =
     false
   )
 
+
+// bool cbs_get_u16(cbs_t *cbs, uint16_t *out)
 val cbs_get_u16 :
   cbs: buffer cbs_t{length cbs = 1} ->
-  out: buffer U16.t{length out = 1} ->
+  out: buffer U16.t{length out = 1 /\ disjoint out cbs} ->
   ST bool
-  (requires (fun h -> live h out /\ live h cbs /\ live h (get h cbs 0).data))
+  (requires (fun h -> live h out /\ live h cbs /\ live h (get h cbs 0).data
+    /\ disjoint out (get h cbs 0).data /\ disjoint cbs (get h cbs 0).data
+  ))
   (ensures (fun h0 r h1 -> live h1 out /\ modifies_1 out h0 h1 /\
     (let cbs0 = get h0 cbs 0 in
       // Return false if there aren't enough bytes.
-      r == (U32.v cbs0.len > 1) //\
+      r == (U32.v cbs0.len > 1) /\
       // If there are, check the result.
-      //(r ==> U16.v (get h1 out 0) == big_endian (slice (as_seq h0 cbs0.data) 0 2))
+      (r ==> U16.v (get h1 out 0) == big_endian (slice (as_seq h0 cbs0.data) 0 2))
     )))
 
 let cbs_get_u16 cbs out =
@@ -105,33 +129,42 @@ let cbs_get_u16 cbs out =
   pop_frame ();
   rv
 
+
+// bool cbs_get_u24(cbs_t *cbs, uint32_t *out)
+// TODO check that it's always < pow2 24
 val cbs_get_u24 :
   cbs: buffer cbs_t{length cbs = 1} ->
-  out: buffer U32.t{length out = 1} ->
+  out: buffer U32.t{length out = 1 /\ disjoint out cbs} ->
   ST bool
-  (requires (fun h -> live h out /\ live h cbs /\ live h (get h cbs 0).data))
+  (requires (fun h -> live h out /\ live h cbs /\ live h (get h cbs 0).data
+    /\ disjoint out (get h cbs 0).data /\ disjoint cbs (get h cbs 0).data
+  ))
   (ensures (fun h0 r h1 -> live h1 out /\ modifies_1 out h0 h1 /\
     (let cbs0 = get h0 cbs 0 in
       // Return false if there aren't enough bytes.
-      r == (U32.v cbs0.len > 2) //\
+      r == (U32.v cbs0.len > 2) /\
       // If there are, check the result.
-      //(r ==> U32.v (get h1 out 0) == big_endian (slice (as_seq h0 cbs0.data) 0 3))
+      (r ==> U32.v (get h1 out 0) == big_endian (slice (as_seq h0 cbs0.data) 0 3))
     )))
 
 let cbs_get_u24 cbs out =
   cbs_get_u cbs out 3ul
 
+
+// bool cbs_get_u32(cbs_t *cbs, uint32_t *out)
 val cbs_get_u32 :
   cbs: buffer cbs_t{length cbs = 1} ->
-  out: buffer U32.t{length out = 1} ->
+  out: buffer U32.t{length out = 1 /\ disjoint out cbs} ->
   ST bool
-  (requires (fun h -> live h out /\ live h cbs /\ live h (get h cbs 0).data))
+  (requires (fun h -> live h out /\ live h cbs /\ live h (get h cbs 0).data
+    /\ disjoint out (get h cbs 0).data /\ disjoint cbs (get h cbs 0).data
+  ))
   (ensures (fun h0 r h1 -> live h1 out /\ modifies_1 out h0 h1 /\
     (let cbs0 = get h0 cbs 0 in
       // Return false if there aren't enough bytes.
-      r == (U32.v cbs0.len > 3) //\
+      r == (U32.v cbs0.len > 3) /\
       // If there are, check the result.
-      //(r ==> U32.v (get h1 out 0) == big_endian (slice (as_seq h0 cbs0.data) 0 4))
+      (r ==> U32.v (get h1 out 0) == big_endian (slice (as_seq h0 cbs0.data) 0 4))
     )))
 
 let cbs_get_u32 cbs out =
